Syntax and semantics of Kore utilising a dependently typed approach (#450)
* Initial generation of Kore

* Add sort axioms to theories

* Fixing Sorts symbol

* Add missing sorted quatifiers

* Kore syntax finished

* Fix proof system names

* wf tactic failure

* Fixes to wf_auto2

* Non-binder Kore wf and simplification classes

* Fix mu, nu according to the PoP paper

* Minor improvements for some equivalence theorems

* Kore fixes (in conj, disj, ceil) + equivalences

* Eq elim in Kore

* Experimental tactics for well-formedness

* Progress with original Kore, start inconsistency issue

* Imp-equiv

* Fix Kore syntax, prove equivalences, start derived rules

* Changed OPMLPattern to be dependent

Also includes temporary example.

* Test for closed pattern

Numbers need to be explicitly written in Check,
might be problematic elsewhere too.

* Investagate unsorted syntax + sorting judgement - substitution

* Fix example (unsorted approach)

* Made closed patterns more usable and renamed them

* Progress with unsorted syntax, dependently-typed semantics

* Consistency proof finished

* Proof of consistency of a forall-based axiom

* Missing file from prev commit, sort inference

* Minor fixes in sort inference

* Kore syntax - first approach

* Eliminate all admits, create general string variable signature

* Sort out Makefile, progress with syntax (sortedness)

* Refactor and extend OPML to Kore (semantics WIP)

* Dep-typed syntax of Kore

* Substitution complete

* Semantics finished

* CI + README

* Typo in Nix flake

* Cleanup

* Remove unnecessary fine

* Fix _CoqProject

* Fix proof system constructor names in prover

* Address comments

---------

Co-authored-by: Kurucz Ádám <cphfw1@inf.elte.hu>

kore/.Makefile.d
@@ -1,0 +1,4 @@
+src/Signature.vo src/Signature.glob src/Signature.v.beautified src/Signature.required_vo: src/Signature.v 
+src/Signature.vos src/Signature.vok src/Signature.required_vos: src/Signature.v 
+src/Syntax.vo src/Syntax.glob src/Syntax.v.beautified src/Syntax.required_vo: src/Syntax.v src/Signature.vo ../matching-logic/src/Utils/extralibrary.vo ../matching-logic/src/Utils/Lattice.vo
+src/Syntax.vos src/Syntax.vok src/Syntax.required_vos: src/Syntax.v src/Signature.vos ../matching-logic/src/Utils/extralibrary.vos ../matching-logic/src/Utils/Lattice.vos
