kore/src/Basics.v
@@ -1,0 +1,146 @@
+From stdpp Require Export list propset.
+From Coq Require Export Program.Equality.
+
+Import ListNotations.
+
+Definition is_leftb {A B : Set} (x : A + B) : bool :=
+match x with
+| inl _ => true
+| _ => false
+end.
+
+Definition is_rightb {A B : Set} (x : A + B) : bool :=
+match x with
+| inl _ => false
+| _ => true
+end.
+
+Definition andb_split_1 (b1 b2 : bool) : andb b1 b2 = true -> b1 = true.
+Proof.
+  destruct b1, b2; simpl; try reflexivity.
+  all: intros; congruence.
+Defined.
+
+Definition andb_split_2 (b1 b2 : bool) : andb b1 b2 = true -> b2 = true.
+Proof.
+  destruct b1, b2; simpl; try reflexivity.
+  all: intros; congruence.
+Defined.
+
+Inductive hlist {A : Type} {F : A -> Type} : list A -> Type :=
+| hnil : hlist []
+| hcons {x : A} {xs : list A} : F x -> hlist xs -> hlist (x :: xs).
+
+Arguments hlist {_} _ & _.
+Arguments hnil {_} {_}.
+Arguments hcons {_} {_} {_} {_} & _ _.
+Arguments hlist_rect {_} {_} {_} & _ _ {_} _ /.
+
+Declare Scope hlist_scope.
+Bind Scope hlist_scope with hlist.
+Delimit Scope hlist_scope with hlist.
+Notation "[ ]" := hnil (format "[ ]") : hlist_scope.
+Notation "[ x ]" := (hcons _ x hnil)  : hlist_scope.
+Notation "[ x ; y ; .. ; z ]" := (hcons x (hcons y .. (hcons z hnil) ..))  : hlist_scope.
+
+Fixpoint pointwise_elem_of {A : Type} {T : A -> Type}
+  ss {struct ss} :
+  (* (l : @hlist A T ss)
+  (lps : @hlist A (fun s => propset (T s)) ss) *)
+  @hlist A T ss ->
+  @hlist A (fun s => propset (T s)) ss ->
+  Prop. (* := *)
+Proof.
+  refine (match ss with
+    | []    => fun _ _ => True
+    | s::ss => fun l l' =>
+      (match l in (@hlist _ _ l1)
+        return (l1 = s::ss -> Prop) with
+      | hnil =>
+        fun (H : [] = s :: ss) => False_rect Prop ltac:(discriminate H)
+      | @hcons _ _ a l0 x xs =>
+        fun (H : a :: l0 = s::ss) =>
+          (match l' in (@hlist _ _ l1')
+             return l1' = s::ss -> Prop with
+           | hnil => fun (H0 : [] = s :: ss) => False_rect Prop ltac:(discriminate H0)
+           | @hcons _ _ a' l0' y ys =>
+             fun (H0 : a' :: l0' = s :: ss) =>
+               x ∈ y /\ pointwise_elem_of _ _ ss _ _
+           end
+          ) eq_refl
+      end) eq_refl
+    end).
+  * injection H. injection H0. intros. rewrite H4. rewrite H2.
+    typeclasses eauto.
+  * injection H. intros. rewrite H1 in xs. exact xs.
+  * injection H0. intros. rewrite H1 in ys. exact ys.
+Defined.
+
+Definition test1 : hlist (bool_rect _ nat bool) [true; false] := [1; true]%hlist.
+Definition test2 : hlist (propset ∘ bool_rect _ nat bool) [true; false] := [{[1]}; {[true]}]%hlist.
+Goal pointwise_elem_of _ test1 test2.
+Proof.
+  simpl. set_solver.
+Qed.
+
+
+Inductive InTy {A : Type} : A -> list A -> Type :=
+  | In_nil {x} {xs} : InTy x (x :: xs)
+  | In_cons {x y} {xs} : InTy y xs -> InTy y (x :: xs)
+.
+
+Definition cons_eq_inv {A : Type} {x y : A} {xs ys : list A}
+  (H : x :: xs = y :: ys) : x = y /\ xs = ys :=
+    conj (f_equal (list_rect _ x (λ a _ _, a)) H)
+         (f_equal (list_rect _ xs (λ _ a _, a)) H).
+
+Fixpoint InTy_app {A : Type} {s : A} {ex ex' ex'' : list A} 
+  (pf : InTy s (ex ++ ex'')) : InTy s (ex ++ ex' ++ ex'').
+Proof.
+  dependent destruction pf.
+  - destruct ex; simpl in *.
+    + induction ex'; simpl.
+      * rewrite <- x. left.
+      * right. exact IHex'.
+    + apply cons_eq_inv in x as [-> ->].
+      left.
+  - destruct ex; simpl in *.
+    + induction ex'; simpl.
+      * rewrite <- x.
+        right. exact pf.
+      * right. exact IHex'.
+    + apply cons_eq_inv in x as [-> ->].
+      right. apply InTy_app. exact pf.
+Defined.
+
+Arguments InTy_app {_} {_} {_} {_} {_} !_.
+
+Definition app_comm_cons_defined
+ : ∀ (A : Type) (x y : list A) (a : A),
+     a :: x ++ y = (a :: x) ++ y.
+Proof.
+  intros. simpl.
+  reflexivity.
+Defined.
+
+Ltac invt H := inversion H; subst; clear H.
+
+Lemma JMeq_eq_rect {U : Type} {P : U → Type} {p q : U} {x : P p} {y : P q} (H : p = q) : JMeq x y -> eq_rect p P x q H = y.
+Proof.
+  intros.
+  apply JMeq_eq_dep, eq_dep_eq_sigT, eq_sigT_sig_eq in H0 as [].
+  rewrite (Eqdep.EqdepTheory.UIP _ _ _ H x0).
+  all: assumption.
+Defined.
+
+
+Create HintDb kore.
+Hint Unfold AntiSymm : kore.
+Hint Constructors PartialOrder : kore.
+Hint Extern 5 (EqDecision _) => unfold EqDecision, Decision; decide equality : kore.
+Hint Unfold eq_rect_r : kore.
+Hint Rewrite -> Eqdep.EqdepTheory.eq_rect_eq : kore.
+Hint Rewrite <- Eqdep.EqdepTheory.eq_rect_eq : kore.
+Hint Unfold Equality.block solution_left : kore.
+Hint Extern 5 (?x ∈ ⊤) => simple apply elem_of_top' : kore.
+Hint Unfold Equality.block solution_left : kore.
