kore/src/Freshness.v
@@ -1,0 +1,64 @@
+From Kore Require Export Syntax.
+
+Section Freshness.
+
+  Context {Σ : Signature}.
+
+  Fixpoint free_evars {ex mu s}
+                      (φ : Pattern ex mu s)
+                      (sTarget : sort) {struct φ} : gset (evar sTarget) :=
+  match φ with
+   | @kore_fevar _ _ _ var_sort x =>
+       (* var_sort = s in this case *)
+       match decide (sTarget = var_sort) with
+       | left H => {[eq_rect_r evar x H]}
+       | right _ => ∅
+       end
+   | kore_imp φ1 φ2 | kore_iff φ1 φ2
+   | kore_and φ1 φ2 | kore_or φ1 φ2
+   | kore_equals _ φ1 φ2 | kore_in _ φ1 φ2
+      => free_evars φ1 sTarget ∪ free_evars φ2 sTarget
+   | kore_app σ args
+      => hlist_rect ∅ (fun _ _ x xs rest => free_evars x sTarget ∪ rest) args
+   | kore_exists _ φ | kore_forall _ φ
+   | kore_mu φ | kore_nu φ 
+   | kore_not φ | kore_ceil _ φ | kore_floor _ φ
+      => free_evars φ sTarget
+   | kore_bevar _ | kore_fsvar _ | kore_bsvar _
+   | kore_bot _ | kore_top _ => ∅
+  end.
+
+  Fixpoint free_svars {ex mu s}
+                      (φ : Pattern ex mu s)
+                      (sTarget : sort) {struct φ} : gset (svar sTarget) :=
+  match φ with
+   | @kore_fsvar _ _ _ var_sort X =>
+       (* var_sort = s in this case *)
+       match decide (sTarget = var_sort) with
+       | left H => {[eq_rect_r svar X H]}
+       | right _ => ∅
+       end
+   | kore_imp φ1 φ2 | kore_iff φ1 φ2
+   | kore_and φ1 φ2 | kore_or φ1 φ2
+   | kore_equals _ φ1 φ2 | kore_in _ φ1 φ2
+      => free_svars φ1 sTarget ∪ free_svars φ2 sTarget
+   | kore_app σ args
+      => hlist_rect ∅ (fun _ _ x xs rest => free_svars x sTarget ∪ rest) args
+   | kore_exists _ φ | kore_forall _ φ
+   | kore_mu φ | kore_nu φ 
+   | kore_not φ | kore_ceil _ φ | kore_floor _ φ
+      => free_svars φ sTarget
+   | kore_bevar _ | kore_fevar _ | kore_bsvar _
+   | kore_bot _ | kore_top _ => ∅
+  end.
+
+  Definition fresh_evar {s} {ex mu}
+      (sTarget : sort) (φ : Pattern s ex mu) :
+      evar sTarget :=
+    fresh (elements (free_evars φ sTarget)).
+  Definition fresh_svar {s} {ex mu}
+      (sTarget : sort) (φ : Pattern s ex mu) :
+      svar sTarget :=
+    fresh (elements (free_svars φ sTarget)).
+
+End Freshness.
