kore/src/Semantics.v
@@ -1,0 +1,178 @@
+From Equations Require Import Equations.
+From Kore Require Export Substitution
+                         Freshness
+                         Basics.
+Require Import Coq.Program.Equality.
+
+
+
+Section Semantics.
+  Context {Σ : Signature}.
+
+  Record Model := {
+    carrier :> sort -> Set;
+    app (σ : symbol) :
+       @hlist _ carrier (arg_sorts σ) -> propset (carrier (ret_sort σ));
+    inhabited (s : sort) : Inhabited (carrier s)
+  }.
+
+  Section with_model.
+
+  Context {M : Model}.
+  Record Valuation : Type := {
+    evar_valuation {s : sort} (x : evar s) : carrier M s;
+    svar_valuation {s : sort} (X : svar s) : propset (carrier M s) ;
+  }.
+
+  Definition app_ext
+    (σ : symbol)
+    (args : @hlist _ (fun s => propset (carrier M s)) (arg_sorts σ))
+    : propset (carrier M (ret_sort σ)) :=
+  PropSet (
+    fun e => exists (l : @hlist _ (carrier M) (arg_sorts σ)),
+      pointwise_elem_of _ l args /\ e ∈ app M σ l
+  ).
+
+
+  Definition update_evar_val {s} (ev : evar s) (x : carrier M s) (val : Valuation) : Valuation.
+  Proof.
+    unshelve esplit.
+    intros s' ev'.
+    destruct (decide (s = s')).
+    destruct (decide (eq_rect s evar ev _ e = ev')).
+    exact (eq_rect s M x _ e).
+    1,2:exact (evar_valuation val ev').
+    exact (@svar_valuation val).
+  Defined.
+
+  Definition update_svar_val {s} (sv : svar s) (X : propset (carrier M s)) (val : Valuation) : Valuation.
+  Proof.
+    unshelve esplit.
+    exact (@evar_valuation val).
+    intros s' sv'.
+    destruct (decide (s = s')).
+    * destruct (decide (eq_rect s svar sv _ e = sv')).
+      - rewrite e in X. exact X.
+      - exact (svar_valuation val sv').
+    * exact (svar_valuation val sv').
+  Defined.
+
+  Let OS s := PropsetOrderedSet (carrier M s).
+  Let  L s := PowersetLattice (carrier M s).
+
+  Equations? eval {ex mu} {s} (ρ : Valuation) (φ : Pattern ex mu s) : propset (carrier M s) by wf (pat_size φ) :=
+    eval ρ (kore_bevar _) := empty ;
+    eval ρ (kore_fevar x) := {[evar_valuation ρ x]} ;
+    eval ρ (kore_bsvar _) := empty ;
+    eval ρ (kore_fsvar X) := svar_valuation ρ X ;
+
+    eval ρ (kore_app σ l) := app_ext σ _ (*@hlist_rect _ _ (λ l _, hlist (propset ∘ M) l) hnil (λ _ _ a _ b, hcons (eval ρ a) b) _ l*) ;
+
+    eval ρ kore_bot         := empty ;
+    eval ρ kore_top         := ⊤ ;
+    eval ρ (kore_not φ)     := ⊤ ∖ (eval ρ φ) ;
+    eval ρ (kore_and φ1 φ2) := (eval ρ φ1) ∩ (eval ρ φ2) ;
+    eval ρ (kore_or φ1 φ2)  := (eval ρ φ1) ∪ (eval ρ φ2) ;
+    eval ρ (kore_imp φ1 φ2) := (⊤ ∖ (eval ρ φ1)) ∪ (eval ρ φ2) ;
+    eval ρ (kore_iff φ1 φ2) := (⊤ ∖ eval ρ φ1 ∪ eval ρ φ2) ∩
+                               (⊤ ∖ eval ρ φ2 ∪ eval ρ φ1) ;
+
+    eval ρ (kore_exists s' φ) := (* ⊤ ≫= λ X, let o := fresh_evar s' φ in eval (update_evar_val o X ρ) (bevar_subst [] φ (kore_fevar o)) *)
+      let x := fresh_evar s' φ in
+        propset_fa_union (λ c,
+           eval (update_evar_val x c ρ)
+                (bevar_subst [] (kore_fevar x) φ)) ;
+    eval ρ (kore_forall s' φ) :=
+      let x := fresh_evar s' φ in
+        propset_fa_intersection (λ c,
+           eval (update_evar_val x c ρ)
+                (bevar_subst [] (kore_fevar x) φ)) ;
+
+(*@LeastFixpointOf _ OS L
+                                  (fun S =>
+                                    let ρ' := (update_svar_val X S ρ) in
+                                    eval ρ' (ϕ'^{svar: 0 ↦ X})
+                                  )*)
+
+    eval ρ (kore_mu φ)     :=
+      let X := fresh_svar s φ in
+        @LeastFixpointOf _ (OS s) (L s) (fun S =>
+          eval (update_svar_val X S ρ)
+               (bsvar_subst [] (kore_fsvar X) φ)
+        )
+     ;
+    eval ρ (kore_nu φ)     :=
+      let X := fresh_svar s φ in
+        @GreatestFixpointOf _ (OS s) (L s) (fun S =>
+          eval (update_svar_val X S ρ)
+               (bsvar_subst [] (kore_fsvar X) φ)
+        );
+
+    eval ρ (kore_ceil φ)       := PropSet (λ _, ∃ c, c ∈ eval ρ φ) ;
+    eval ρ (kore_floor φ)      := PropSet (λ _, ∀ c, c ∈ eval ρ φ) ;
+    eval ρ (kore_equals φ1 φ2) := PropSet (λ _, (eval ρ φ1) = (eval ρ φ2)) ;
+    eval ρ (kore_in φ1 φ2)     := PropSet (λ _, (eval ρ φ1) ⊆ (eval ρ φ2)) ;
+  .
+  Proof.
+    1: {
+      simpl in *.
+      induction l.
+      * exact hnil.
+      * apply hcons.
+        - apply (eval _ _ _ ρ f). lia.
+        - apply IHl. intros.
+          apply (eval x0 x1 x2 x3 x4). lia.
+    }
+    all: try by simpl; lia.
+    1-2: rewrite (bevar_subst_size [] ex mu s s' φ x); constructor.
+    1-2: rewrite (bsvar_subst_size ex [] mu s s φ X); constructor.
+  Defined.
+
+  Definition satM {ex mu s} (φ : Pattern ex mu s) :=
+    forall ρ, eval ρ φ ≡ ⊤.
+
+  Definition satT (Γ : Theory) :=
+    forall p, p ∈ Γ -> @satM _ _ (projT1 p) (projT2 p).
+
+  Import PropExtensionality.
+  #[export]
+  Instance propset_leibniz_equiv A : LeibnizEquiv (propset A).
+  Proof.
+    intros x y H. unfold equiv in H. unfold set_equiv_instance in H.
+    destruct x,y.
+    apply f_equal. apply functional_extensionality.
+    intros x. apply propositional_extensionality.
+    specialize (H x). destruct H as [H1 H2].
+    split; auto.
+  Qed.
+
+(*   Fixpoint HForall {J} {A : J -> Type}
+    (P : ∀ j, A j -> Prop)
+    {js : list J} (v : @hlist J A js) {struct v} : Prop :=
+    match v with
+    | hnil => True
+    | hcons x xs => P _ x ∧ HForall P xs
+    end.
+
+  Fixpoint HBiForall {J1 J2} {A1 : J1 -> Type} {A2 : J2 -> Type}
+    (P : ∀ j1 j2, A1 j1 -> A2 j2 -> Prop)
+    {js1 : list J1}
+    {js2 : list J2}
+    (v1 : @hlist J1 A1 js1) (v2 : @hlist J2 A2 js2)
+      {struct v1} : Prop :=
+    match v1, v2 with
+    | hnil, hnil => True
+    | hcons x xs, hcons y ys => P _ _ x y ∧ HBiForall P xs ys
+    | _, _ => False
+    end.
+
+  Fixpoint hmap {J} {A B : J -> Type}
+    (f : ∀ j, A j -> B j)
+    {js : list J} (v : @hlist J A js) : @hlist J B js :=
+  match v with
+  | hnil => hnil
+  | hcons x xs => hcons (f _ x) (hmap f xs)
+  end. *)
+
+End with_model.
+End Semantics.
