kore/src/Signature.v
@@ -1,0 +1,69 @@
+From Coq Require Export ssreflect ssrfun ssrbool String.
+From stdpp Require Export
+  base
+  countable
+  infinite.
+
+
+Set Default Proof Mode "Classic".
+
+Class Sorts := {
+    sort : Set;
+    sort_eqdec :: EqDecision sort;
+    sort_countable :: Countable sort;
+(*     subsort : relation sort;
+    subsort_po :: PartialOrder subsort; *)
+}.
+
+(* Class Variables {Ss : Sorts} := {
+  evar : Set;
+  svar : Set;
+  evar_eqdec :: EqDecision evar;
+  evar_countable :: Countable evar;
+  (* evar_infinite :: Infinite evar; *)
+  svar_eqdec :: EqDecision svar;
+  svar_countable :: Countable svar;
+  (* svar_infinite :: Infinite svar; *)
+
+  evar_sort : evar -> sort;
+  svar_sort : svar -> sort;
+
+  evar_infinite s ::
+    Infinite {x : evar & decide (evar_sort x = s)};
+  svar_infinite s ::
+    Infinite {x : svar & decide (svar_sort x = s)}
+}. *)
+
+Class Variables {Ss : Sorts} := {
+  evar : sort -> Set;
+  svar : sort -> Set;
+  evar_eqdec :: forall s, EqDecision (evar s);
+  evar_countable :: forall s, Countable (evar s);
+  evar_infinite :: forall s, Infinite (evar s);
+  svar_eqdec :: forall s, EqDecision (svar s);
+  svar_countable :: forall s, Countable (svar s);
+  svar_infinite :: forall s, Infinite (svar s);
+}.
+
+Class Symbols {Ss : Sorts} := {
+  symbol : Set;
+  sym_eqdec :: EqDecision symbol;
+  sym_countable :: Countable symbol;
+  arg_sorts : symbol -> list sort ;
+  ret_sort : symbol -> sort ;
+}.
+
+Class Signature := {
+  sorts :: Sorts ;
+  variables :: Variables;
+  symbols :: Symbols;
+}.
+
+Module StringVariables.
+  Program Instance StringVariables {Ss : Sorts} : Variables := {|
+    evar := fun _ => string;
+    svar := fun _ => string;
+  |}.
+  Fail Next Obligation.
+
+End StringVariables.
