kore/src/Substitution.v
@@ -1,0 +1,409 @@
+From Kore Require Export Syntax Freshness.
+
+Import Kore.Syntax.Notations.
+
+Tactic Notation "hlist_map" uconstr(f) "in" ident(h) :=
+  let y := fresh in let H := fresh in
+  induction h as [ | ? ? y _ H];
+  [left | right];
+  [eapply f; eauto using y | exact H].
+
+Tactic Notation "hlist_foldr" uconstr(f) "with" uconstr(def) "in" ident(h) :=
+let y := fresh in let H := fresh in
+  induction h as [ | ?x ?xs y _ H ];
+  [exact def | eapply f];
+  [exact y | exact H].
+
+Section Substitution.
+  Context {Σ : Signature}.
+
+  Fixpoint inc_var {ex ex' ex'' mu mu' mu''} {s}
+    (base : Pattern (ex ++ ex'') (mu ++ mu'') s)
+    : Pattern (ex ++ ex' ++ ex'') (mu ++ mu' ++ mu'') s.
+  Proof.
+    revert s ex ex' ex'' mu mu' mu'' base.
+    fix IH 8.
+    intros.
+    dependent destruction base.
+    - apply kore_bevar, InTy_app, idx.
+    - apply kore_bsvar, InTy_app, idx.
+    - apply kore_fevar, x.
+    - apply kore_fsvar, X.
+    - apply kore_app.
+      (* hlist_map inc_evar in h. *)
+      (* epose proof (@hlist_rect _ _
+        (fun l => hlist _ l) hnil). *)
+      (* refine (hlist_rect []%hlist
+            (fun _ _ x xs rest => _) args). *)
+      hlist_map inc_var in args.
+    (* bot *)
+    - exact (kore_bot s).
+    (* top *)
+    - exact (kore_top s).
+    (* not *)
+    - apply kore_not; apply inc_var.
+      exact base.
+    (* and *)
+    - apply kore_and; apply inc_var.
+      exact base1. exact base2.
+    (* or *)
+    - apply kore_or; apply inc_var.
+      exact base1. exact base2.
+    (* imp *)
+    - apply kore_imp; apply inc_var.
+      exact base1. exact base2.
+    (* iff *)
+    - apply kore_iff; apply inc_var.
+      exact base1. exact base2.
+    (* exists *)
+    - eapply kore_exists. instantiate (1 := s_var).
+      rewrite app_comm_cons_defined.
+      apply inc_var.
+      rewrite <- app_comm_cons_defined.
+      exact base.
+    (* forall *)
+    - eapply kore_forall. instantiate (1 := s_var).
+      rewrite app_comm_cons_defined.
+      apply inc_var.
+      rewrite <- app_comm_cons_defined.
+      exact base.
+    (* mu *)
+    - eapply kore_mu.
+      rewrite app_comm_cons_defined.
+      apply inc_var.
+      rewrite <- app_comm_cons_defined.
+      exact base.
+    (* nu *)
+    - eapply kore_nu.
+      rewrite app_comm_cons_defined.
+      apply inc_var.
+      rewrite <- app_comm_cons_defined.
+      exact base.
+    (* ceil *)
+    - eapply kore_ceil; apply inc_var.
+      exact base.
+    (* floor *)
+    - eapply kore_floor; apply inc_var.
+      exact base.
+    (* equals *)
+    - eapply kore_equals; apply inc_var.
+      exact base1. exact base2.
+    (* in *)
+    - eapply kore_in; apply inc_var.
+      exact base1. exact base2.
+  Defined.
+
+  Arguments inc_var {_} {_} {_} {_} {_} {_} {_} !_.
+
+  (*
+  The following two function substitute the `(length ex)`th index in the dB index
+  `idx` by `ψ`. The result is likely a `kore_bevar idx` (`kore_bsvar dbi` resp.),
+  except when `idx` is the `(length ex)`th index, in which case it is ψ, with its
+  context extended with `ex`.
+  *)
+  Fixpoint sub_evar {s s'} {ex ex' mu}
+    (idx : InTy s (ex ++ s' :: ex'))
+    (ψ : Pattern ex' mu s') {struct idx}
+      : Pattern (ex ++ ex') mu s.
+  Proof.
+    refine (match idx in (InTy o l) return (o = s -> l = ex ++ s' :: ex' -> Pattern (ex ++ ex') mu s) with
+            | In_nil => _
+            | In_cons idx => _
+            end eq_refl eq_refl); intros; subst.
+    - destruct ex; simpl in *; apply cons_eq_inv in H0 as [-> ->].
+      + exact ψ.
+      + apply kore_bevar, In_nil.
+    - destruct ex; simpl in *; apply cons_eq_inv in H0 as [-> ->].
+      + apply kore_bevar, idx.
+      + specialize (sub_evar _ _ _ _ _ idx ψ).
+        apply (@inc_var [] [s1] (ex ++ ex') [] [] mu _).
+        simpl. exact sub_evar.
+  Defined.
+
+  Arguments sub_evar {_} {_} {_} {_} {_} !_ _.
+
+  Fixpoint sub_svar {s s'} {ex mu mu'}
+    (dbi : InTy s (mu ++ s' :: mu'))
+    (ψ : Pattern ex mu' s') {struct dbi}
+    : Pattern ex (mu ++ mu') s.
+  Proof.
+    refine (match dbi in (InTy o l) return (o = s -> l = mu ++ s' :: mu' -> Pattern ex (mu ++ mu') s) with
+            | In_nil => _
+            | In_cons idx => _
+            end eq_refl eq_refl); intros; subst.
+    - destruct mu; simpl in *; apply cons_eq_inv in H0 as [-> ->].
+      + exact ψ.
+      + apply kore_bsvar, In_nil.
+    - destruct mu; simpl in *; apply cons_eq_inv in H0 as [-> ->].
+      + apply kore_bsvar, idx.
+      + specialize (sub_svar _ _ _ _ _ idx ψ).
+        apply (@inc_var [] [] ex [] [s1] (mu ++ mu')).
+        simpl. exact sub_svar.
+  Defined.
+
+  Arguments sub_svar {_} {_} {_} {_} {_} !_ _.
+
+  Fixpoint bevar_subst ex {ex' mu : list sort} {s s'}
+    (ψ : Pattern ex' mu s')
+    (φ : Pattern (ex ++ s' :: ex') mu s) {struct φ}
+    : Pattern (ex ++ ex') mu s.
+  Proof.
+    intros.
+    dependent destruction φ.
+    (* bevar *)
+    - eapply sub_evar; eauto.
+    (* bsvar *)
+    - apply kore_bsvar. exact idx.
+    (* fevar *)
+    - apply kore_fevar, x.
+    (* fsvar *)
+    - apply kore_fsvar, X.
+    (* app *)
+    - apply kore_app.
+      hlist_map bevar_subst in args.
+    (* bot *)
+    - exact (kore_bot s).
+    (* top *)
+    - exact (kore_top s).
+    (* not *)
+    - exact (kore_not (bevar_subst _ _ _ _ _ ψ φ)).
+    (* and *)
+    - exact (kore_and (bevar_subst _ _ _ _ _ ψ φ1)
+                      (bevar_subst _ _ _ _ _ ψ φ2)).
+    (* or *)
+    - exact (kore_or (bevar_subst _ _ _ _ _ ψ φ1)
+                     (bevar_subst _ _ _ _ _ ψ φ2)).
+    (* imp *)
+    - exact (kore_imp (bevar_subst _ _ _ _ _ ψ φ1)
+                      (bevar_subst _ _ _ _ _ ψ φ2)).
+    (* iff *)
+    - exact (kore_iff (bevar_subst _ _ _ _ _ ψ φ1)
+                      (bevar_subst _ _ _ _ _ ψ φ2)).
+    (* exists *)
+    - eapply kore_exists.
+      rewrite app_comm_cons_defined.
+      eapply bevar_subst. exact ψ.
+      rewrite <- app_comm_cons_defined. exact φ.
+    (* forall *)
+    - eapply kore_forall.
+      rewrite app_comm_cons_defined.
+      eapply bevar_subst. exact ψ.
+      rewrite <- app_comm_cons_defined. exact φ.
+    (* mu *)
+    - eapply kore_mu.
+      eapply bevar_subst. 2: exact φ.
+      apply (@inc_var [] [] ex' [] [s] mu s').
+      assumption.
+    (* nu *)
+    - eapply kore_nu.
+      eapply bevar_subst. 2: exact φ.
+      apply (@inc_var [] [] ex' [] [s] mu s').
+      assumption.
+    (* ceil *)
+    - eapply kore_ceil.
+      eapply bevar_subst.
+      exact ψ. exact φ.
+    (* floor *)
+    - eapply kore_ceil.
+      eapply bevar_subst.
+      exact ψ. exact φ.
+    (* equals *)
+    - exact (kore_equals _ (bevar_subst _ _ _ _ _ ψ φ1)
+                      (bevar_subst _ _ _ _ _ ψ φ2)).
+    (* in *)
+    - exact (kore_in _ (bevar_subst _ _ _ _ _ ψ φ1)
+                      (bevar_subst _ _ _ _ _ ψ φ2)).
+  Defined.
+
+  Arguments bevar_subst _ {_} {_} {_} {_} !_ _.
+
+
+  Fixpoint bsvar_subst {ex} mu {mu' : list sort} {s s'}
+    (ψ : Pattern ex mu' s')
+    (φ : Pattern ex (mu ++ s'::mu') s) {struct φ}
+    : Pattern ex (mu ++ mu') s.
+  Proof.
+    intros.
+    dependent destruction φ.
+    (* bevar *)
+    - eapply kore_bevar. exact idx.
+    (* bsvar *)
+    - eapply sub_svar; eauto.
+    (* fevar *)
+    - apply kore_fevar, x.
+    (* fsvar *)
+    - apply kore_fsvar, X.
+    (* app *)
+    - apply kore_app.
+      hlist_map bsvar_subst in args.
+    (* bot *)
+    - exact (kore_bot s).
+    (* top *)
+    - exact (kore_top s).
+    (* not *)
+    - exact (kore_not (bsvar_subst _ _ _ _ _ ψ φ)).
+    (* and *)
+    - exact (kore_and (bsvar_subst _ _ _ _ _ ψ φ1)
+                      (bsvar_subst _ _ _ _ _ ψ φ2)).
+    (* or *)
+    - exact (kore_or (bsvar_subst _ _ _ _ _ ψ φ1)
+                     (bsvar_subst _ _ _ _ _ ψ φ2)).
+    (* imp *)
+    - exact (kore_imp (bsvar_subst _ _ _ _ _ ψ φ1)
+                      (bsvar_subst _ _ _ _ _ ψ φ2)).
+    (* iff *)
+    - exact (kore_iff (bsvar_subst _ _ _ _ _ ψ φ1)
+                      (bsvar_subst _ _ _ _ _ ψ φ2)).
+    (* exists *)
+    - eapply kore_exists.
+      eapply bsvar_subst. 2: exact φ.
+      apply (@inc_var [] [s_var] ex [] [] mu' s').
+      assumption.
+    (* forall *)
+    - eapply kore_forall.
+      eapply bsvar_subst. 2: exact φ.
+      apply (@inc_var [] [s_var] ex [] [] mu' s').
+      assumption.
+    (* mu *)
+    - eapply kore_mu.
+      rewrite app_comm_cons_defined.
+      eapply bsvar_subst. exact ψ.
+      rewrite <- app_comm_cons_defined. exact φ.
+    (* nu *)
+    - eapply kore_nu.
+      rewrite app_comm_cons_defined.
+      eapply bsvar_subst. exact ψ.
+      rewrite <- app_comm_cons_defined. exact φ.
+    (* ceil *)
+    - eapply kore_ceil.
+      eapply bsvar_subst.
+      exact ψ. exact φ.
+    (* floor *)
+    - eapply kore_ceil.
+      eapply bsvar_subst.
+      exact ψ. exact φ.
+    (* equals *)
+    - exact (kore_equals _ (bsvar_subst _ _ _ _ _ ψ φ1)
+                      (bsvar_subst _ _ _ _ _ ψ φ2)).
+    (* in *)
+    - exact (kore_in _ (bsvar_subst _ _ _ _ _ ψ φ1)
+                      (bsvar_subst _ _ _ _ _ ψ φ2)).
+  Defined.
+
+  Arguments bevar_subst {_} _ {_} {_} {_} !_ _.
+
+End Substitution.
+
+Module Notations.
+
+  Notation "p '^[' 'evar:' s ↦ t ']'" :=
+    (bevar_subst s t p) : kore_scope.
+  Notation "p '^[' 'svar:' s ↦ t ']'" :=
+    (bsvar_subst s t p) : kore_scope.
+
+End Notations.
+
+Section Substitution.
+  Import Notations.
+
+  Context {Σ : Signature}.
+
+  Lemma inc_var_size : forall s ex ex' ex'' mu mu' mu'' (φ : Pattern (ex ++ ex'') (mu ++ mu'') s),
+    pat_size (@inc_var Σ ex ex' ex'' mu mu' mu'' s φ) =
+    pat_size φ.
+  Proof.
+    fix IH 8. intros.
+    dependent destruction φ; try reflexivity.
+    all: simpl; try by auto.
+    - simpl. induction args.
+      * by auto.
+      * simpl. rewrite IH. by auto.
+    - cbn.
+      specialize (IH s (s_var :: ex) ex' ex'' mu mu' mu'' φ).
+      f_equal. assumption.
+    - cbn.
+      specialize (IH s (s_var :: ex) ex' ex'' mu mu' mu'' φ).
+      f_equal. assumption.
+    - cbn.
+      specialize (IH s ex ex' ex'' (s :: mu) mu' mu'' φ).
+      f_equal. assumption.
+    - cbn.
+      specialize (IH s ex ex' ex'' (s :: mu) mu' mu'' φ).
+      f_equal. assumption.
+  Defined.
+
+  Lemma sub_evar_size s s' ex ex' mu o idx:
+    pat_size (@sub_evar Σ s s' ex ex' mu idx (kore_fevar o)) = 1.
+  Proof.
+    dependent induction ex; simpl in *.
+    * dependent destruction idx; cbn; reflexivity.
+    * dependent destruction idx; cbn. reflexivity.
+      epose proof inc_var_size _ [] [a] (ex ++ ex') [] [] mu (sub_evar idx (kore_fevar o)).
+      rewrite IHex in H.
+      exact H.
+  Defined.
+
+  Lemma bevar_subst_size : forall ex ex' mu s s'
+    (φ : Pattern (ex ++ s' :: ex') mu s)
+    o,
+      pat_size (bevar_subst ex (kore_fevar o) φ) =
+      pat_size φ.
+  Proof.
+    fix IH 6.
+    intros.
+    dependent destruction φ; simpl; try reflexivity.
+    all: try by auto.
+    - autounfold with kore.
+      simpl. clear IH.
+      apply sub_evar_size.
+    - induction args; simpl.
+      + reflexivity.
+      + simpl. by auto.
+    - specialize (IH (s_var :: ex) ex' mu s s').
+      cbn. by f_equal.
+    - specialize (IH (s_var :: ex) ex' mu s s').
+      cbn. by f_equal.
+    - specialize (IH ex ex' (s :: mu) s s').
+      cbn. by f_equal.
+    - specialize (IH ex ex' (s :: mu) s s').
+      cbn. by f_equal.
+  Defined.
+
+  Lemma sub_svar_size s s' ex mu mu' o idx:
+    pat_size (@sub_svar Σ s s' ex mu mu' idx (kore_fsvar o)) = 1.
+  Proof.
+    dependent induction mu; simpl in *.
+    * dependent destruction idx; cbn; reflexivity.
+    * dependent destruction idx; cbn. reflexivity.
+      epose proof inc_var_size _ [] [] ex [] [a] (mu ++ mu') (sub_svar idx (kore_fsvar o)).
+      rewrite IHmu in H.
+      exact H.
+  Defined.
+
+  Lemma bsvar_subst_size : forall ex mu mu' s s'
+    (φ : Pattern ex (mu ++ s' :: mu') s)
+    o,
+      pat_size (bsvar_subst mu (kore_fsvar o) φ) =
+      pat_size φ.
+  Proof.
+    fix IH 6.
+    intros.
+    dependent destruction φ; simpl; try reflexivity.
+    all: try by auto.
+    - autounfold with kore.
+      simpl. clear IH.
+      apply sub_svar_size.
+    - induction args; simpl.
+      + reflexivity.
+      + simpl. by auto.
+    - specialize (IH (s_var :: ex) mu mu' s s').
+      cbn. by f_equal.
+    - specialize (IH (s_var :: ex) mu mu' s s').
+      cbn. by f_equal.
+    - specialize (IH ex (s :: mu) mu' s s').
+      cbn. by f_equal.
+    - specialize (IH ex (s :: mu) mu' s s').
+      cbn. by f_equal.
+  Defined.
+
+End Substitution.
