matching-logic/src/Experimental/Kore_alternative.v
@@ -1,0 +1,1220 @@
+From MatchingLogic Require Export ProofMode.MLPM
+                                  FOEquality_ProofSystem
+                                  Sorts_ProofSystem.
+From MatchingLogic.Theories Require Export Nat_Syntax.
+
+Import MatchingLogic.Logic.Notations.
+Import MatchingLogic.Theories.Definedness_Syntax.Notations.
+Import MatchingLogic.Theories.Sorts_Syntax.Notations.
+Import MatchingLogic.Theories.Nat_Syntax.Notations.
+
+Set Default Proof Mode "Classic".
+
+(* For the well-formedness tactics, we forbid simplifications *)
+Arguments well_formed_positive : simpl never.
+Arguments well_formed_closed_mu_aux : simpl never.
+Arguments well_formed_closed_ex_aux : simpl never.
+
+Inductive Symbols := kore_next_symbol | kore_dv_symbol | kore_inj_symbol.
+
+#[global]
+Instance Symbols_eqdec: EqDecision Symbols.
+Proof.
+    solve_decision.
+Defined.
+
+#[global]
+Program Instance Symbols_finite: Finite Symbols :=
+{|
+  enum := [kore_next_symbol;kore_dv_symbol;kore_inj_symbol]
+|}.
+Next Obligation.
+    compute_done.
+Qed.
+Next Obligation.
+    destruct x; compute_done.
+Qed.
+
+#[global]
+Instance Symbols_countable : countable.Countable Symbols.
+Proof. apply finite.finite_countable. Defined.
+
+Section derived_operations.
+  Context {Σ : Signature}.
+
+  Class Syntax :=
+    { sym_inj : Symbols -> symbols;
+      imported_sorts : Sorts_Syntax.Syntax; (* TODO: this might change based on the formalisation of built-ins! *)
+    }.
+
+  #[global] Existing Instance imported_definedness.
+  #[global] Existing Instance imported_sorts.
+
+  Context {self : Syntax}.
+  Definition kore_sym (s : Symbols) : Pattern := patt_sym (sym_inj s).
+
+  (* TODO: check if s is needed! *)
+  Definition kore_bottom (s : Pattern) := patt_bott.
+  #[global]
+  Program Instance kore_bottom_Nullary s : Nullary (kore_bottom s).
+  Next Obligation.
+    intros. rewrite pm_correctness. simpl. reflexivity.
+  Defined.
+  Solve Obligations of kore_bottom_Nullary with intros;wf_auto2.
+  Fail Next Obligation.
+
+  Definition kore_top (s : Pattern) := patt_inhabitant_set s.
+  #[global]
+  Program Instance kore_top_Unary : Unary kore_top.
+  Next Obligation.
+    intros. rewrite pm_correctness. simpl.
+    rewrite pm_correctness. reflexivity.
+  Defined.
+  Solve Obligations of kore_top_Unary with intros;wf_auto2.
+  Fail Next Obligation.
+
+  Definition kore_cast (s p : Pattern) :=
+    patt_and p (kore_top s).
+  #[global]
+  Program Instance kore_cast_Binary : Binary kore_cast.
+  Next Obligation.
+    intros. repeat rewrite pm_correctness. simpl.
+    repeat rewrite pm_correctness. reflexivity.
+  Defined.
+  Solve Obligations of kore_cast_Binary with intros; unfold kore_cast; wf_auto2.
+  Fail Next Obligation.
+
+  Definition kore_valid (s : Pattern) (ph1 : Pattern) :=
+    patt_equal ph1 (kore_top s).
+  #[global]
+  Program Instance kore_top_Binary : Binary kore_valid.
+  Next Obligation.
+    intros. repeat rewrite pm_correctness. simpl.
+    repeat rewrite pm_correctness. reflexivity.
+  Defined.
+  Solve Obligations of kore_top_Binary with intros; unfold kore_valid; wf_auto2.
+  Fail Next Obligation.
+
+  Definition kore_not (s : Pattern) (ph1 : Pattern) :=
+    kore_cast s (patt_not ph1).
+  #[global]
+  Program Instance kore_not_Binary : Binary kore_not.
+  Next Obligation.
+    intros. repeat rewrite pm_correctness. simpl.
+    repeat rewrite pm_correctness. reflexivity.
+  Defined.
+  Solve Obligations of kore_not_Binary with intros; unfold kore_not; wf_auto2.
+  Fail Next Obligation.
+
+  (* NOTE: this is changed wrt MM *)
+  Definition kore_and (s : Pattern) (ph1 : Pattern) (ph2 : Pattern) :=
+    kore_cast s (patt_and ph1 ph2).
+  #[global]
+  Program Instance kore_and_Ternary : Ternary kore_and.
+  Next Obligation.
+    intros. repeat rewrite pm_correctness. simpl.
+    repeat rewrite pm_correctness. reflexivity.
+  Defined.
+  Solve Obligations of kore_and_Ternary with intros; unfold kore_and; wf_auto2.
+  Fail Next Obligation.
+
+  Local Goal forall φ1 s, well_formed φ1 -> well_formed s -> well_formed (kore_and s φ1 ⊥).
+  Proof.
+    intros. wf_auto2.
+  Qed.
+
+  (* NOTE: this is changed wrt MM *)
+  Definition kore_or (s : Pattern) (ph1 : Pattern) (ph2 : Pattern) :=
+    kore_cast s (patt_or ph1 ph2).
+  #[global]
+  Program Instance kore_or_Ternary : Ternary kore_or.
+  Next Obligation.
+    intros. rewrite pm_correctness. simpl.
+    repeat rewrite pm_correctness. reflexivity.
+  Defined.
+  Solve Obligations of kore_or_Ternary with intros; unfold kore_or; wf_auto2.
+  Fail Next Obligation.
+
+  Local Goal forall φ1 s, well_formed φ1 -> well_formed s -> well_formed (kore_or s φ1 ⊥).
+  Proof.
+    intros. wf_auto2.
+  Qed.
+
+
+  Definition kore_implies (s : Pattern) (ph1 : Pattern) (ph2 : Pattern) :=
+    kore_or s (kore_not s ph1) ph2.
+  #[global]
+  Program Instance kore_implies_Ternary : Ternary kore_implies.
+  Next Obligation.
+    intros. repeat rewrite pm_correctness. simpl.
+    repeat rewrite pm_correctness. reflexivity.
+  Defined.
+  Solve Obligations of kore_implies_Ternary with intros; unfold kore_implies; wf_auto2.
+  Fail Next Obligation.
+
+  Local Goal forall φ1, well_formed φ1 -> well_formed (kore_implies (p_x) φ1 ⊥).
+  Proof.
+    intros. wf_auto2.
+  Qed.
+
+  Definition kore_iff (s : Pattern) (ph1 : Pattern) (ph2 : Pattern) :=
+    kore_and s (kore_implies s ph1 ph2) (kore_implies s ph2 ph1).
+  #[global]
+  Program Instance kore_iff_Ternary : Ternary kore_iff.
+  Next Obligation.
+    intros. repeat rewrite pm_correctness. simpl.
+    repeat rewrite pm_correctness. reflexivity.
+  Defined.
+  Solve Obligations of kore_iff_Ternary with intros; unfold kore_iff; wf_auto2.
+  Fail Next Obligation.
+
+  Local Goal forall φ1, well_formed φ1 -> well_formed (kore_iff (p_x) φ1 ⊥).
+  Proof.
+    intros. wf_auto2.
+  Qed.
+
+  (* TODO: check if s1 is needed!
+     TODO: this seems to be wrong. s1 is not used for ph2!
+  *)
+  Definition kore_ceil (s1 : Pattern) (s2 : Pattern) (ph2 : Pattern) := 
+    kore_cast s2 (patt_defined (kore_cast s1 ph2)).
+  #[global]
+  Program Instance kore_ceil_Ternary : Ternary kore_ceil.
+  Next Obligation.
+    intros. repeat rewrite pm_correctness. simpl.
+    repeat rewrite pm_correctness. reflexivity.
+  Defined.
+  Solve Obligations of kore_ceil_Ternary with intros; unfold kore_ceil; wf_auto2.
+  Fail Next Obligation.
+  Local Goal forall s1 s2 φ1, well_formed φ1 -> well_formed s1 -> well_formed s2 -> well_formed (kore_ceil s1 s2 φ1).
+  Proof.
+    intros. wf_auto2.
+  Qed.
+
+
+  Definition kore_floor (s1 : Pattern) (s2 : Pattern) (ph2 : Pattern) := 
+    kore_not s2 (kore_ceil s1 s2 (kore_not s1 ph2)).
+  #[global]
+  Program Instance kore_floor_Ternary : Ternary kore_floor.
+  Next Obligation.
+    intros. repeat rewrite pm_correctness. simpl.
+    repeat rewrite pm_correctness. reflexivity.
+  Defined.
+  Solve Obligations of kore_floor_Ternary with intros; unfold kore_floor; wf_auto2.
+  Fail Next Obligation.
+
+  Local Goal forall s2 φ1, well_formed φ1 -> well_formed s2 -> well_formed (kore_floor ⊥ s2 φ1).
+  Proof.
+    intros. wf_auto2.
+  Qed.
+
+  Definition kore_equals (s1 : Pattern) (s2 : Pattern) (ph2 : Pattern) (ph3: Pattern) := 
+    kore_floor s1 s2 (kore_iff s1 ph2 ph3).
+  #[global]
+  Program Instance kore_equals_Quaternary : Quaternary kore_equals.
+  Next Obligation.
+    intros. repeat rewrite pm_correctness. simpl.
+    repeat rewrite pm_correctness. reflexivity.
+  Defined.
+  Solve Obligations of kore_equals_Quaternary with intros; unfold kore_equals; wf_auto2.
+  Fail Next Obligation.
+
+  Local Goal forall s2 φ1 φ2,
+    well_formed φ1 ->
+    well_formed s2 ->
+    well_formed φ2 -> well_formed (kore_equals s2 Top φ1 φ2).
+  Proof.
+    intros. wf_auto2.
+  Qed.
+
+  (* Q: why not kore_ceil and conjunction? *)
+  (* A: because this is not kore-in, but rather kore-subseteq *)
+  Definition kore_in (s1 : Pattern) (s2 : Pattern) (ph2 : Pattern) (ph3: Pattern) := 
+    kore_floor s1 s2 (kore_implies s1 ph2 ph3).
+  #[global]
+  Program Instance kore_in_Quaternary : Quaternary kore_in.
+  Next Obligation.
+    intros. repeat rewrite pm_correctness. simpl.
+    repeat rewrite pm_correctness. reflexivity.
+  Defined.
+  Solve Obligations of kore_in_Quaternary with intros; unfold kore_in; wf_auto2.
+  Fail Next Obligation.
+
+  Local Goal forall s2 φ1 φ2,
+    well_formed φ1 ->
+    well_formed s2 ->
+    well_formed φ2 -> well_formed (kore_in s2 Top φ1 φ2).
+  Proof.
+    intros. wf_auto2.
+  Qed.
+
+  (*
+    TODO:
+    the following constructs do not match into the
+    class scheme described in SyntacticConstruct.v!
+  *)
+
+  Definition kore_exists (s1 : Pattern) (s2 : Pattern) (ph2 : Pattern) :=
+    kore_cast s2 (patt_sorted_exists s1 ph2).
+  Definition kore_forall (s1 : Pattern) (s2 : Pattern) (ph2 : Pattern) :=
+    kore_not s2 (kore_exists s1 s2 (kore_not s2 ph2)).
+(*   Definition kore_forall_sort (s : Pattern) :=
+    patt_forall_sort s. *)
+  Definition kore_is_sort (s : Pattern) := patt_exists_sort (patt_equal b0 (nest_ex s)).
+  (* #[global]
+  Program Instance kore_is_sort_Unary : Unary kore_is_sort.
+  Next Obligation.
+    intros. unfold kore_is_sort.
+    rewrite ebinder_morphism.
+    rewrite binary_morphism.
+    f_equal. f_equal.
+    rewrite pm_correctness. simpl. by rewrite pm_ezero_increase.
+    Search nest_ex increase_ex.
+  Defined.
+  Solve Obligations of kore_top_Unary with intros;wf_auto2.
+  Fail Next Obligation. *)
+
+
+  Definition kore_is_predicate (s : Pattern) (ph1 : Pattern) :=
+    patt_or (kore_valid s ph1) (patt_equal ph1 patt_bott).
+  Definition kore_is_nonempty_sort (s : Pattern) :=
+    patt_defined (kore_top s).
+
+  (* These are just ml primitives *)
+  Definition kore_mu := patt_mu.
+  Definition kore_nu := patt_nu.
+
+  Definition kore_next (s : Pattern) (ph1 : Pattern) :=
+    patt_app (kore_sym kore_next_symbol) ph1.
+  Definition kore_all_path_next (s : Pattern) (ph1 : Pattern) :=
+    kore_not s (kore_next s (kore_not s ph1)).
+  Definition kore_eventually (s : Pattern) (ph1 : Pattern) :=
+    kore_mu (kore_or (nest_mu s) (nest_mu ph1) (kore_next (nest_mu s) B0)).
+  (* TODO: check. not well_founded and eventually is equivalent to this: *)
+  Definition kore_weak_eventually (s : Pattern) (ph1 : Pattern) :=
+    kore_not s (kore_mu (kore_not (nest_mu s)
+                             (kore_or (nest_mu s)
+                                      (nest_mu ph1)
+                                      (kore_next (nest_mu s)
+                                        (kore_not (nest_mu s) B0))))).
+  Definition kore_always (s : Pattern) (ph1 : Pattern) := 
+    kore_not s (kore_mu (kore_not (nest_mu s)
+       (kore_and (nest_mu s) (nest_mu ph1)
+         (kore_all_path_next (nest_mu s) (kore_not (nest_mu s) B0))))).
+  Definition kore_well_founded (s : Pattern) :=
+    kore_mu (kore_all_path_next (nest_mu s) B0).
+  Definition kore_well_founded_alt (s : Pattern) :=
+    kore_mu (kore_all_path_next (nest_mu s) (kore_always (nest_mu s) B0)).
+  Definition kore_rewrites (s : Pattern) (ph1 : Pattern) (ph2 : Pattern) :=
+    kore_implies s ph1 (kore_next s ph2).
+  Definition kore_rewrites_star (s : Pattern) (ph1 : Pattern) (ph2 : Pattern) :=
+    kore_implies s ph1 (kore_eventually s ph2).
+  Definition kore_rewrites_plus (s : Pattern) (ph1 : Pattern) (ph2 : Pattern) :=
+    kore_implies s ph1 (kore_next s (kore_eventually s ph2)).
+
+
+  Definition kore_one_path_reaches_star (s : Pattern) (ph1 : Pattern) (ph2 : Pattern) :=
+    kore_implies s ph1 (kore_weak_eventually s ph2).
+  Definition kore_one_path_reaches_plus (s : Pattern) (ph1 : Pattern) (ph2 : Pattern) :=
+    kore_implies s ph1 (kore_next s (kore_weak_eventually s ph2)).
+  Definition kore_circularity (s : Pattern) (ph1 : Pattern) :=
+    kore_all_path_next s (kore_always s ph1).
+  Definition kore_non_terminating (s : Pattern) := kore_next s (kore_top s).
+
+  Definition kore_all_path_next_nt (s : Pattern) (ph1 : Pattern) :=
+    kore_and s (kore_all_path_next s ph1) (kore_non_terminating s).
+  Definition kore_all_path_eventually (s : Pattern) (ph1 : Pattern) :=
+    kore_mu (kore_or (nest_mu s) (nest_mu ph1) (kore_all_path_next_nt (nest_mu s) B0)).
+  Definition kore_all_path_rewrites (s : Pattern) (ph1 : Pattern) (ph2 : Pattern) :=
+    kore_implies s ph1 (kore_all_path_next_nt s ph2).
+  Definition kore_all_path_rewrites_star (s : Pattern) (ph1 : Pattern) (ph2 : Pattern) :=
+    kore_implies s ph1 (kore_all_path_eventually s ph2).
+  Definition kore_all_path_rewrites_plus (s : Pattern) (ph1 : Pattern) (ph2 : Pattern) :=
+    kore_implies s ph1 (kore_all_path_next_nt s (kore_all_path_eventually s ph2)).
+
+  Definition kore_dv (ph0 : Pattern) (ph1 : Pattern) :=
+    patt_app (patt_app (kore_sym kore_dv_symbol) ph0) ph1.
+
+
+  Definition kore_inj (s1 : Pattern) (s2 : Pattern) (ph2 : Pattern) :=
+    patt_app (patt_app (patt_app (kore_sym kore_inj_symbol) s1) s2) ph2.
+
+  (**
+    Things to consider:
+    - From where can we omit the sorts?
+    - Related to that: Which constructs can be expressed in a more simple form with more
+      primitive ML constructs? That would significantly improve the usability of Kore without
+      proving additional derived properties.
+    - kore_well_founded <---> kore_well_founded_alt?
+  *)
+
+(*   Next Obligation.
+  admit.
+  Admitted.
+  Next Obligation.
+  admit.
+  Admitted.
+Next Obligation.
+  admit.
+  Admitted.
+  Next Obligation.
+  admit.
+  Admitted. *)
+
+
+
+End derived_operations.
+
+Module Notations.
+
+  (* NOTE: format attribute is needed to avoid unnecessary whitespaces *)
+  Notation "'⊥(' s ')'" := (kore_bottom s) (format "'⊥(' s ')'") : ml_scope.
+  Check ⊥(Nat).
+  Notation "'Top(' s ')'" := (kore_top s) (format "'Top(' s ')'") : ml_scope.
+  Check Top(Nat).
+  Notation "p ∷ s" := (kore_cast s p) (at level 65, format "p  ∷  s", right associativity).
+  Check Zero ∷ Nat.
+  Notation "'⊢(' s ')' p" := (kore_valid s p) (at level 80, format "'⊢(' s ')'  p").
+  Check ⊢(Nat) ⊥.
+  Notation "'!(' s ')' p" := (kore_not s p) (at level 71, format "'!(' s ')'  p") : ml_scope.
+  Check !(Nat) ⊥.
+  Notation "p1 'and(' s ')' p2" := (kore_and s p1 p2) (at level 72, format "p1  'and(' s ')'  p2", left associativity) : ml_scope.
+  Check ⊥ and(Nat) Top.
+  Notation "p1 'or(' s ')' p2" := (kore_or s p1 p2) (at level 73, format "p1  'or(' s ')'  p2", left associativity) : ml_scope.
+  Check ⊥ or(Nat) Top.
+  Notation "p1 '-(' s ')->' p2" := (kore_implies s p1 p2) (at level 75, format "p1  '-(' s ')->'  p2", right associativity) : ml_scope.
+  Check ⊥ -(Nat)-> Top.
+  Notation "p1 '<-(' s ')->' p2" := (kore_iff s p1 p2) (at level 74, format "p1  '<-(' s ')->'  p2") : ml_scope.
+  Check ⊥ <-(Nat)-> Top.
+
+  Notation "'⌈(' s1 , s2 ')' p ⌉" := (kore_ceil s1 s2 p) (format "'⌈(' s1 ',' s2 ')'  p ⌉") : ml_scope.
+  Check ⌈(Nat, Nat) ⊥⌉.
+  Notation "'⌊(' s1 , s2 ')' p ⌋" := (kore_floor s1 s2 p) (format "'⌊(' s1 ',' s2 ')'  p ⌋") : ml_scope.
+  Check ⌊(Nat, Nat) ⊥⌋.
+  Notation "p1 '=ml(' s1 ',' s2 ')' p2" := (kore_equals s1 s2 p1 p2) (at level 68, format "p1  '=ml(' s1 ',' s2 ')'  p2", left associativity) : ml_scope.
+  Check ⊥ =ml(Nat, Nat) Top.
+  Notation "p1 '⊆ml(' s1 ',' s2 ')' p2" := (kore_in s1 s2 p1 p2) (at level 68, format "p1  '⊆ml(' s1 ',' s2 ')'  p2", left associativity) : ml_scope.
+  Check ⊥ ⊆ml(Nat, Nat) Top.
+
+  Notation "'ex' s1 ',' p 'as' s2" := (kore_exists s1 s2 p) (at level 80, s2 at level 65, format "'ex'  s1 ','  p  'as'  s2") : ml_scope.
+  Check ex Nat , ⊥ as Nat.
+  Notation "'all' s1 ',' p 'as' s2" := (kore_forall s1 s2 p) (at level 80, s2 at level 65, format "'all'  s1 ','  p  'as'  s2") : ml_scope.
+  Goal forall {Σ : Signature} {s1 : Syntax} {s2 : Nat_Syntax.Syntax},
+    ~ (all Nat , ⊥ as Nat ⋅ Nat) = (all Nat , ⊥ as (Nat ⋅ Nat)).
+  Proof. intros. intro. inversion H. Qed.
+
+(*   Notation "''" := (kore_is_sort s).
+  Notation := (kore_is_predicate s p).
+  Notation := (kore_is_nonempty_sort s). *)
+
+  (* Notation "'mu' s , p" := (kore_mu s p) (at level 80).
+  Check mu Nat, ⊥.
+  Notation "'nu' s , p" := (kore_nu s p) (at level 80).
+  Check nu Nat, ⊥. *)
+
+  Notation "'•(' s ')' p"    := (kore_next s p) (at level 30, format "'•(' s ')'  p") : ml_scope.
+  Check •(Nat) ⊥.
+  Notation "'○(' s ')' p"    := (kore_all_path_next s p) (at level 71, format "'○(' s ')'  p") : ml_scope.
+  Check ○(Nat) ⊥.
+  Notation "'⋄(' s ')' p"    := (kore_eventually s p) (at level 71, format "'⋄(' s ')'  p") : ml_scope.
+  Check ⋄(Nat) ⊥.
+  Notation "'⋄ʷ(' s ')' p"   := (kore_weak_eventually s p) (at level 71, format "'⋄ʷ(' s ')'  p") : ml_scope.
+  Check ⋄ʷ(Nat) ⊥.
+(*   Notation "s"       := (kore_well_founded s) (at level 71) : ml_scope. *)
+(*   Notation ""       := (kore_well_founded_alt s) (at level 71) : ml_scope. *)
+  Notation "'⊞(' s ')' p"    := (kore_always s p) (at level 71, format "'⊞(' s ')'  p") : ml_scope. (* □ is taken by application contexts *)
+  Check ⊞(Nat) ⊥.
+  Notation "p '=(' s ')=>' q"  := (kore_rewrites s p q) (at level 81, format "p  '=(' s ')=>'  q") : ml_scope.
+  Check ⊥ =(Nat)=> Top.
+  Notation "p '=(' s ')=>*' q" := (kore_rewrites_star s p q) (at level 81, format "p  '=(' s ')=>*'  q") : ml_scope.
+  Check ⊥ =(Nat)=>* Top.
+  Notation "p '=(' s ')=>⁺' q" := (kore_rewrites_plus s p q) (at level 81, format "p  '=(' s ')=>⁺'  q") : ml_scope.
+  Check ⊥ =(Nat)=>⁺ Top.
+
+(* These probably don't need notations:
+  Notation "" := (kore_one_path_reaches_star s p1 p2).
+  Notation := (kore_one_path_reaches_plus s p1 p2). *)
+  Notation "'↺(' s ')' p" := (kore_circularity s p) (at level 71, format "'↺(' s ')'  p").
+  Check ↺(Nat) ⊥.
+  Notation "s ⇑" := (kore_non_terminating s) (at level 90).
+  Check ⊥ ⋅ ⊥ ⇑.
+
+  (* Notation := (kore_all_path_next_nt s p).
+  Notation := (kore_all_path_eventually s p).
+  Notation := (kore_all_path_rewrites s p1 p2).
+  Notation := (kore_all_path_rewrites_star s p1 p2).
+  Notation := (kore_all_path_rewrites_plus s p1 p2).
+
+  Notation := (kore_dv p1 p2).
+  Notation := (kore_inj s1 s2 p). *)
+
+End Notations.
+
+Section KoreTheory.
+
+  Import Notations.
+  Context
+    {Σ : Signature}
+    {syntax : Syntax}
+  .
+
+ (*  Inductive AxiomName : Set :=
+  | InjId
+  | SortNext
+  | SortDv.
+
+  Print kore_dv. *)
+  (* REMARK: all of these three axioms from Metamath seem to be too strong. Quantification is
+     missing! *)
+(*   Definition axiom (name : AxiomName) : Pattern :=
+  match name with
+  (* kore-inj-id $a |- ( \eq ( \kore-inj ph0 ph1 ph2 ) ph2 ) $. *)
+  | InjId => allₛ, allₛ, all b1, kore_inj b2 b1 b0 =ml b0
+  (* kore-next-sorting $a |- ( \imp ( \in-sort ph1 ph0 ) ( \in-sort ( \kore-next ph0 ph1 ) ph0 ) ) $. *)
+  | SortNext => allₛ, all b0, b0 ⊆ml ⟦b1⟧ ---> •(b1) b0 ⊆ml ⟦b1⟧
+  (* kore-dv-sorting $a |- ( \in-sort ( \kore-dv ph0 ph1 ) ph0 ) $. *)
+  | SortDv => allₛ, all b0, kore_dv b1 b0 ⊆ml ⟦b1⟧
+  (*
+    ∀s : Sorts, ∀x : s, kore_dv x s ∈ ⟦s⟧
+    kore-dv ph0 ph1 ⊆ ⟦ph0⟧
+  *)
+  end.
+  Eval simpl in axiom InjId.
+  Eval simpl in axiom SortNext.
+  Eval simpl in axiom SortDv. *)
+
+  Inductive AxiomName : Set :=
+  | InjId φ1 φ2 φ3 : well_formed φ1 -> well_formed φ2 -> well_formed φ3 -> AxiomName
+  | SortNext φ1 φ2 : well_formed φ1 -> well_formed φ2 -> AxiomName
+  | SortDv φ1 φ2 : well_formed φ1 -> well_formed φ2 -> AxiomName.
+
+  Definition axiom (name : AxiomName) : Pattern :=
+  match name with
+  (* kore-inj-id $a |- ( \eq ( \kore-inj ph0 ph1 ph2 ) ph2 ) $. *)
+  | InjId φ0 φ1 φ2 _ _ _ => kore_inj φ0 φ1 φ2 =ml φ2
+  (* kore-next-sorting $a |- ( \imp ( \in-sort ph1 ph0 ) ( \in-sort ( \kore-next ph0 ph1 ) ph0 ) ) $. *)
+  | SortNext φ0 φ1 _ _ => φ1 ⊆ml ⟦φ0⟧ ---> •(φ0) φ1 ⊆ml ⟦φ0⟧
+  (* kore-dv-sorting $a |- ( \in-sort ( \kore-dv ph0 ph1 ) ph0 ) $. *)
+  | SortDv φ0 φ1 _ _ => kore_dv φ0 φ1 ⊆ml ⟦φ0⟧
+  (*
+    ∀s : Sorts, ∀x : s, kore_dv x s ∈ ⟦s⟧
+    kore-dv ph0 ph1 ⊆ ⟦ph0⟧
+  *)
+  end.
+  Eval simpl in axiom (InjId ⊥ ⊥ ⊥ ltac:(wf_auto2) ltac:(wf_auto2) ltac:(wf_auto2)).
+  Eval simpl in axiom (SortNext ⊥ ⊥ ltac:(wf_auto2) ltac:(wf_auto2)).
+  Eval simpl in axiom (SortDv ⊥ ⊥ ltac:(wf_auto2) ltac:(wf_auto2)).
+
+  Program Definition named_axioms : NamedAxioms :=
+    {|
+      NAName := AxiomName;
+      NAAxiom := axiom;
+    |}.
+  Next Obligation.
+    destruct name; simpl; unfold kore_inj, kore_dv; wf_auto2.
+  Defined.
+
+  Definition KoreTheory := Definedness_Syntax.theory ∪
+                           theory_of_NamedAxioms named_axioms.
+
+  Local Goal KoreTheory ⊢ kore_dv ⊥ Top ⊆ml ⟦⊥⟧.
+  Proof.
+    gapply hypothesis. 2: wf_auto2. try_solve_pile.
+    unfold KoreTheory.
+    unfold theory_of_NamedAxioms.
+    apply elem_of_union_r.
+    exists (SortDv ⊥ Top ltac:(wf_auto2) ltac:(wf_auto2)). set_solver.
+  Qed.
+
+End KoreTheory.
+
+Section Lemmas.
+
+(*   Require Import wftacticsoriginal. *)
+(* Arguments well_formed_positive /.
+Arguments well_formed_closed_mu_aux /.
+Arguments well_formed_closed_ex_aux /. *)
+  Import Notations.
+  Context
+    {Σ : Signature}
+    {syntax : Syntax}
+    (Γ : Theory)
+    (HΓ : KoreTheory ⊆ Γ)
+  .
+
+  Lemma implies_equiv_1 :
+    forall s φ ψ,
+      well_formed s ->
+      well_formed φ ->
+      well_formed ψ ->
+      Γ ⊢ (φ -(s)-> ψ) ---> (φ ---> ψ) ∷ s.
+  Proof.
+    intros. mlIntro "H".
+    mlDestructAnd "H" as "H1" "H2".
+    mlSplitAnd. 2: mlAssumption.
+    mlIntro "H3".
+    mlDestructOr "H1" as "H" "H". 2: mlAssumption.
+    mlDestructAnd "H" as "H0" "H1".
+    mlApply "H0" in "H3". mlDestructBot "H3".
+  Defined.
+
+  Lemma implies_equiv_2 :
+    forall s φ ψ,
+      well_formed s ->
+      well_formed φ ->
+      well_formed ψ ->
+      Γ ⊢ (φ ---> ψ) ∷ s ---> (φ -(s)-> ψ).
+  Proof.
+    intros.
+    mlIntro "H".
+    mlDestructAnd "H" as "H1" "H2".
+    mlSplitAnd. 2: mlAssumption.
+    mlIntro "H3".
+    mlApplyMeta deMorgan_nand_1 in "H3".
+    mlDestructOr "H3" as "H" "H".
+    * mlApply "H1". mlApplyMeta not_not_elim in "H".
+      mlAssumption.
+    * mlExFalso. mlApply "H". mlAssumption.
+  Defined.
+
+  Theorem implies_equiv :
+    forall s φ ψ,
+      well_formed s ->
+      well_formed φ ->
+      well_formed ψ ->
+      Γ ⊢ (φ -(s)-> ψ) <---> (φ ---> ψ) ∷ s.
+  Proof.
+    intros.
+    mlSplitAnd.
+    * mlIntro. mlApplyMeta implies_equiv_1. mlAssumption.
+    * mlIntro. mlApplyMeta implies_equiv_2. mlAssumption.
+  Defined.
+
+  Lemma iff_equiv_1 :
+    forall s φ ψ,
+      well_formed s ->
+      well_formed φ ->
+      well_formed ψ ->
+      Γ ⊢ (φ <-(s)-> ψ) ---> ((φ <---> ψ) ∷ s).
+  Proof.
+    intros. unfold kore_iff.
+    pose proof implies_equiv s φ ψ H H0 H1 as HH.
+    pose proof implies_equiv s ψ φ H H1 H0 as FF.
+    mlRewrite HH at 1.
+    mlRewrite FF at 1.
+    unfold kore_and.
+    mlIntro "H"; mlDestructAnd "H".
+    all: mlSplitAnd; try mlAssumption.
+    mlDestructAnd "0". mlDestructAnd "2".
+    mlDestructAnd "3". mlSplitAnd; mlAssumption.
+  Defined.
+
+  Lemma iff_equiv_2 :
+    forall s φ ψ,
+      well_formed s ->
+      well_formed φ ->
+      well_formed ψ ->
+      Γ ⊢ (φ <---> ψ) ∷ s ---> (φ <-(s)-> ψ).
+  Proof.
+    intros. unfold kore_iff.
+    pose proof implies_equiv s φ ψ H H0 H1 as HH.
+    pose proof implies_equiv s ψ φ H H1 H0 as FF.
+    mlRewrite HH at 1.
+    mlRewrite FF at 1.
+    unfold kore_and.
+    mlIntro "H". mlDestructAnd "H" as "H1" "H2".
+    mlDestructAnd "H1".
+    repeat mlSplitAnd; try mlAssumption.
+  Defined.
+
+  Theorem iff_equiv :
+    forall s φ ψ,
+      well_formed s ->
+      well_formed φ ->
+      well_formed ψ ->
+      Γ ⊢ (φ <-(s)-> ψ) <---> (φ <---> ψ) ∷ s.
+  Proof.
+    intros.
+    mlSplitAnd.
+    * mlIntro. mlApplyMeta iff_equiv_1. mlAssumption.
+    * mlIntro. mlApplyMeta iff_equiv_2. mlAssumption.
+  Defined.
+
+  Lemma valid_equiv_1 :
+    forall s φ ψ,
+      well_formed s ->
+      well_formed φ ->
+      well_formed ψ ->
+      Γ ⊢ (⊢(s) φ <-(s)-> ψ) ---> (φ ∷ s =ml ψ ∷ s).
+  Proof.
+    intros. unfold kore_valid.
+    pose proof (iff_equiv s φ ψ H H0 H1).
+    mlRewrite H2 at 1.
+    mlIntro "H".
+    mlApplyMeta patt_total_and_2.
+    2: unfold KoreTheory in HΓ; set_solver.
+    mlSplitAnd.
+    * mlApplyMeta floor_monotonic. mlExact "H".
+      2: wf_auto2.
+      2: unfold KoreTheory in HΓ; set_solver.
+      clear hasserted.
+      instantiate (1 := AnyReasoning).
+      mlIntro "H".
+      mlIntro "H0".
+      mlDestructAnd "H0" as "H0_1" "H0_2".
+      mlSplitAnd. 2: mlAssumption.
+      mlDestructAnd "H" as "H_1" "H_2".
+      mlApply "H_2" in "H0_2".
+      mlDestructAnd "H0_2" as "H3" "H4".
+      mlDestructAnd "H3" as "H5" "H6".
+      mlApply "H5".
+      mlAssumption.
+    * mlApplyMeta floor_monotonic. mlExact "H".
+      2: wf_auto2.
+      2: unfold KoreTheory in HΓ; set_solver.
+      clear hasserted.
+      instantiate (1 := AnyReasoning).
+      mlIntro "H".
+      mlIntro "H0".
+      mlDestructAnd "H0" as "H0_1" "H0_2".
+      mlSplitAnd. 2: mlAssumption.
+      mlDestructAnd "H" as "H_1" "H_2".
+      mlApply "H_2" in "H0_2".
+      mlDestructAnd "H0_2" as "H3" "H4".
+      mlDestructAnd "H3" as "H5" "H6".
+      mlApply "H6".
+      mlAssumption.
+  Defined.
+
+  Lemma valid_equiv_2 :
+    forall s φ ψ,
+      well_formed s ->
+      well_formed φ ->
+      well_formed ψ ->
+      Γ ⊢ (φ ∷ s =ml ψ ∷ s) ---> (⊢(s) φ <-(s)-> ψ).
+  Proof.
+    intros. unfold kore_valid.
+    pose proof (iff_equiv s φ ψ H H0 H1).
+    mlRewrite H2 at 1.
+    mlIntro "H".
+    mlApplyMeta patt_total_and_2.
+    2: unfold KoreTheory in HΓ; set_solver.
+    mlSplitAnd.
+    * mlApplyMeta floor_monotonic. mlExact "H".
+      2: wf_auto2.
+      2: unfold KoreTheory in HΓ; set_solver.
+      clear hasserted.
+      instantiate (1 := AnyReasoning).
+      mlIntro "H".
+      mlIntro "H0".
+      mlDestructAnd "H0" as "H0_1" "H0_2".
+      mlAssumption.
+    * mlApplyMeta floor_monotonic. mlExact "H".
+      2: wf_auto2.
+      2: unfold KoreTheory in HΓ; set_solver.
+      clear hasserted.
+      instantiate (1 := AnyReasoning).
+      mlIntro "H".
+      mlIntro "H0".
+      mlDestructAnd "H" as "H_1" "H_2".
+      mlSplitAnd. 2: mlAssumption.
+      mlSplitAnd.
+      - mlIntro "H".
+        mlConj "H" "H0" as "H2".
+        fold (φ ∷ s).
+        mlApply "H_1" in "H2".
+        mlDestructAnd "H2".
+        mlAssumption.
+      - mlIntro "H".
+        mlConj "H" "H0" as "H2".
+        fold (ψ ∷ s).
+        mlApply "H_2" in "H2".
+        mlDestructAnd "H2".
+        mlAssumption.
+  Defined.
+
+  Theorem valid_equiv :
+    forall s φ ψ,
+      well_formed s ->
+      well_formed φ ->
+      well_formed ψ ->
+      Γ ⊢ (⊢(s) φ <-(s)-> ψ) <---> (φ ∷ s =ml ψ ∷ s).
+  Proof.
+    intros.
+    mlSplitAnd.
+    * mlIntro. mlApplyMeta valid_equiv_1. mlAssumption.
+    * mlIntro. mlApplyMeta valid_equiv_2. mlAssumption.
+  Defined.
+
+  Lemma floor_equiv_1 :
+    forall s1 s2 φ,
+      well_formed s1 ->
+      well_formed s2 ->
+      well_formed φ ->
+      Γ ⊢ ⌊(s1, s2) φ⌋ ---> ⌊φ or !Top(s1)⌋ ∷ s2.
+  Proof.
+    intros.
+    unfold kore_floor, kore_ceil, kore_not.
+    mlIntro "H".
+    mlDestructAnd "H" as "H1" "H2".
+    mlSplitAnd. 2: mlAssumption.
+    unfold patt_total.
+    mlApplyMeta deMorgan_nand_1 in "H1".
+    mlDestructOr "H1" as "H" "H".
+    2: { mlApply "H" in "H2". mlDestructBot "H2". }
+    mlClear "H2".
+    mlIntro "H0".
+    mlApply "H". mlClear "H".
+    mlApplyMeta ceil_monotonic. mlAssumption.
+    2: wf_auto2.
+    2: unfold KoreTheory in HΓ; set_solver.
+    instantiate (1 := AnyReasoning).
+    mlIntro "H".
+    mlApplyMeta deMorgan_nor_1 in "H".
+    mlDestructAnd "H" as "H1" "H2".
+    mlApplyMeta not_not_elim in "H2".
+    repeat mlSplitAnd; mlAssumption.
+  Defined.
+
+  Lemma floor_equiv_2 :
+    forall s1 s2 φ,
+      well_formed s1 ->
+      well_formed s2 ->
+      well_formed φ ->
+      Γ ⊢ ⌊φ or !Top(s1)⌋ ∷ s2 ---> ⌊(s1, s2) φ⌋.
+  Proof.
+    intros.
+    unfold kore_floor, kore_ceil, kore_not.
+    mlIntro "H".
+    mlDestructAnd "H" as "H1" "H2".
+    mlSplitAnd. 2: mlAssumption.
+    mlIntro "H". mlDestructAnd "H" as "H0" "H3".
+    mlApply "H1".
+    mlApplyMeta ceil_monotonic. mlExact "H0".
+    2: wf_auto2.
+    2: unfold KoreTheory in HΓ; set_solver.
+    instantiate (1 := AnyReasoning).
+    mlIntro "H".
+    mlIntro "H0".
+    mlDestructAnd "H" as "H1" "H2".
+    mlDestructAnd "H1" as "H3" "H4".
+    mlDestructOr "H0" as "H5" "H5".
+    * mlApply "H3". mlAssumption.
+    * mlApply "H5". mlAssumption.
+  Defined.
+
+  Theorem floor_equiv :
+    forall s1 s2 φ,
+      well_formed s1 ->
+      well_formed s2 ->
+      well_formed φ ->
+      Γ ⊢ ⌊(s1, s2) φ⌋ <---> ⌊φ or !Top(s1)⌋ ∷ s2.
+  Proof.
+    intros.
+    mlSplitAnd.
+    * mlIntro. mlApplyMeta floor_equiv_1. mlAssumption.
+    * mlIntro. mlApplyMeta floor_equiv_2. mlAssumption.
+  Defined.
+
+  Lemma equals_equiv_1 :
+    forall s1 s2 φ ψ,
+      well_formed s1 ->
+      well_formed s2 ->
+      well_formed φ ->
+      well_formed ψ ->
+      Γ ⊢ φ =ml(s1,s2) ψ ---> ((φ ∷ s1) =ml (ψ ∷ s1)) ∷ s2.
+  Proof.
+    intros.
+    unfold kore_equals.
+    mlIntro "H".
+    mlApplyMeta floor_equiv_1 in "H".
+    mlDestructAnd "H" as "H0" "H1".
+    mlSplitAnd. 2: mlAssumption.
+    mlClear "H1".
+    mlApplyMeta floor_monotonic. mlExact "H0".
+    2: wf_auto2.
+    2: unfold KoreTheory in HΓ; set_solver.
+    instantiate (1 := AnyReasoning).
+    mlIntro "H".
+    mlSplitAnd; mlIntro "H0";
+      mlDestructAnd "H0" as "H0_1" "H0_2";
+      mlDestructOr "H" as "H1" "H1".
+    * mlApplyMeta iff_equiv_1 in "H1".
+      mlDestructAnd "H1" as "H2" "H3".
+      mlDestructAnd "H2" as "H4" "H5".
+      mlApply "H4" in "H0_1".
+      mlSplitAnd; mlAssumption.
+    * mlApply "H1" in "H0_2".
+      mlDestructBot "H0_2".
+    * mlApplyMeta iff_equiv_1 in "H1".
+      mlDestructAnd "H1" as "H2" "H3".
+      mlDestructAnd "H2" as "H4" "H5".
+      mlApply "H5" in "H0_1".
+      mlSplitAnd; mlAssumption.
+    * mlApply "H1" in "H0_2".
+      mlDestructBot "H0_2".
+  Defined.
+
+  Lemma equals_equiv_2 :
+    forall s1 s2 φ ψ,
+      well_formed s1 ->
+      well_formed s2 ->
+      well_formed φ ->
+      well_formed ψ ->
+      Γ ⊢ ((φ ∷ s1) =ml (ψ ∷ s1)) ∷ s2 ---> φ =ml(s1,s2) ψ.
+  Proof.
+    intros.
+    mlIntro "H".
+    mlApplyMeta floor_equiv_2.
+    mlDestructAnd "H" as "H0" "H1".
+    mlSplitAnd. 2: mlAssumption.
+    mlApplyMeta floor_monotonic. mlExact "H0".
+    2: wf_auto2.
+    2: unfold KoreTheory in HΓ; set_solver.
+    instantiate (1 := AnyReasoning).
+    mlIntro "H".
+    mlDestructAnd "H" as "H0" "H1".
+    mlIntro "H". mlIntro "H2".
+    mlApply "H".
+    mlApplyMeta iff_equiv_2.
+    mlSplitAnd. 2: mlAssumption.
+    mlSplitAnd; mlIntro "H3"; mlConj "H3" "H2" as "D".
+    * fold (φ ∷ s1).
+      mlApply "H0" in "D". mlDestructAnd "D". mlAssumption.
+    * fold (ψ ∷ s1).
+      mlApply "H1" in "D". mlDestructAnd "D". mlAssumption.
+  Defined.
+
+  Theorem equals_equiv :
+    forall s1 s2 φ ψ,
+      well_formed s1 ->
+      well_formed s2 ->
+      well_formed φ ->
+      well_formed ψ ->
+      Γ ⊢ φ =ml(s1,s2) ψ <--->
+          ((φ ∷ s1) =ml (ψ ∷ s1)) ∷ s2.
+  Proof.
+    intros.
+    mlSplitAnd.
+    * mlIntro. mlApplyMeta equals_equiv_1. mlAssumption.
+    * mlIntro. mlApplyMeta equals_equiv_2. mlAssumption.
+  Defined.
+
+  Lemma in_equiv_1 :
+    forall s1 s2 φ ψ,
+      well_formed s1 ->
+      well_formed s2 ->
+      well_formed φ ->
+      well_formed ψ ->
+      Γ ⊢ φ ⊆ml(s1,s2) ψ ---> ((φ ∷ s1) ⊆ml (ψ ∷ s1)) ∷ s2.
+  Proof.
+    intros.
+    unfold kore_equals.
+    mlIntro "H".
+    mlApplyMeta floor_equiv_1 in "H".
+    mlDestructAnd "H" as "H0" "H1".
+    mlSplitAnd. 2: mlAssumption.
+    mlClear "H1".
+    mlApplyMeta floor_monotonic. mlExact "H0".
+    2: wf_auto2.
+    2: unfold KoreTheory in HΓ; set_solver.
+    instantiate (1 := AnyReasoning).
+    mlIntro "H".
+    mlIntro "H0".
+    mlDestructAnd "H0" as "H1" "H2".
+    mlDestructOr "H" as "H0" "H0".
+    2: { mlApply "H0" in "H2". mlDestructBot "H2". }
+    mlApplyMeta implies_equiv_1 in "H0".
+    mlDestructAnd "H0" as "H" "H3".
+    mlApply "H" in "H1".
+    mlSplitAnd; mlAssumption.
+  Defined.
+
+  Lemma in_equiv_2 :
+    forall s1 s2 φ ψ,
+      well_formed s1 ->
+      well_formed s2 ->
+      well_formed φ ->
+      well_formed ψ ->
+      Γ ⊢ ((φ ∷ s1) ⊆ml (ψ ∷ s1)) ∷ s2 ---> φ ⊆ml(s1,s2) ψ.
+  Proof.
+    intros.
+    mlIntro "H".
+    mlApplyMeta floor_equiv_2.
+    mlDestructAnd "H" as "H0" "H1".
+    mlSplitAnd. 2: mlAssumption.
+    mlApplyMeta floor_monotonic. mlExact "H0".
+    2: wf_auto2.
+    2: unfold KoreTheory in HΓ; set_solver.
+    instantiate (1 := AnyReasoning).
+    mlIntro "H".
+    mlIntro "H0".
+    mlIntro "H1".
+    mlApply "H0".
+    mlApplyMeta implies_equiv_2.
+    mlSplitAnd. 2: mlAssumption.
+    mlIntro "H2".
+    mlConj "H2" "H1" as "D".
+    fold (φ ∷ s1).
+    mlApply "H" in "D".
+    mlDestructAnd "D".
+    mlAssumption.
+  Defined.
+
+  Theorem in_equiv :
+    forall s1 s2 φ ψ,
+      well_formed s1 ->
+      well_formed s2 ->
+      well_formed φ ->
+      well_formed ψ ->
+      Γ ⊢ φ ⊆ml(s1,s2) ψ <---> ((φ ∷ s1) ⊆ml (ψ ∷ s1)) ∷ s2.
+  Proof.
+    intros.
+    mlSplitAnd.
+    * mlIntro. mlApplyMeta in_equiv_1. mlAssumption.
+    * mlIntro. mlApplyMeta in_equiv_2. mlAssumption.
+  Defined.
+
+  Lemma forall_equiv_1 :
+    forall s1 s2 φ,
+      well_formed s1 ->
+      well_formed s2 ->
+      well_formed (ex, φ) ->
+      Γ ⊢ all s1, φ as s2 ---> (all s1 , φ) ∷ s2.
+  Proof.
+    intros.
+    unfold kore_forall, kore_not, kore_exists, kore_top.
+    toMLGoal. { unfold kore_forall, kore_exists, patt_sorted_forall, patt_sorted_exists. wf_auto2. }
+    mlIntro.
+    mlDestructAnd "0".
+    mlSplitAnd. 2: mlAssumption.
+    mlIntroAll x. mlSimpl. cbn.
+    setoid_rewrite nest_ex_same.
+    mlIntro.
+    epose proof deMorgan_nand Γ (ex s1, ! φ and ⟦ s2 ⟧) ⟦ s2 ⟧ _ _.
+    use AnyReasoning in H2.
+    mlAdd H2 as "H2".
+    mlDestructAnd "H2". mlClear "4".
+    mlApply "3" in "1". mlClear "3".
+    mlDestructOr "1".
+    - mlSpecialize "3" with x.
+      mlSimpl. simpl.
+      setoid_rewrite nest_ex_same.
+      rewrite (evar_open_not_occur _ _ s2). wf_auto2.
+      mlDestructOr "3".
+      + mlApply "1" in "0". mlDestructBot "0".
+      + pose proof deMorgan_nand Γ
+            (! φ^{evar:0↦x}) ⟦ s2 ⟧
+       ltac:(wf_auto2) ltac:(wf_auto2).
+       use AnyReasoning in H3.
+       mlAdd H3 as "H3".
+       mlDestructAnd "H3". mlClear "3".
+       mlApply "1" in "4". mlClear "1".
+       mlDestructOr "4".
+       ** mlApplyMeta Misc.notnot_taut_1 in "1".
+          mlAssumption.
+       ** mlApply "3" in "2". mlDestructBot "2".
+    - mlExFalso. mlApply "4". mlAssumption.
+    Unshelve.
+      all: unfold patt_sorted_exists in *; wf_auto2.
+  Defined.
+
+  Lemma forall_equiv_2 :
+    forall s1 s2 φ,
+      well_formed s1 ->
+      well_formed s2 ->
+      well_formed (ex, φ) ->
+      Γ ⊢ (all s1 , φ) ∷ s2 --->  all s1 , φ as s2.
+  Proof.
+    intros.
+    toMLGoal. { unfold kore_forall, kore_exists, patt_sorted_forall, patt_sorted_exists. wf_auto2. }
+    mlIntro. mlDestructAnd "0" as "H" "Hs".
+    mlSplitAnd. 2: mlAssumption.
+    mlIntro "E". mlDestructAnd "E" as "E1" "E2".
+    mlDestructEx "E1" as x.
+    mlSimpl.
+    setoid_rewrite nest_ex_same.
+    rewrite (evar_open_not_occur _ _ s2). wf_auto2.
+    mlDestructAnd "E1" as "E1_1" "E1_2".
+    mlDestructAnd "E1_2".
+    mlApply "0".
+    mlSpecialize "H" with x. mlSimpl. simpl.
+    setoid_rewrite nest_ex_same.
+    mlApply "H". mlAssumption.
+  Defined.
+
+  Theorem forall_equiv :
+    forall s1 s2 φ,
+      well_formed s1 ->
+      well_formed s2 ->
+      well_formed (ex, φ) ->
+      Γ ⊢ all s1, φ as s2 <---> (all s1 , φ) ∷ s2.
+  Proof.
+    intros.
+    toMLGoal. { unfold kore_forall, kore_exists, patt_sorted_forall, patt_sorted_exists. wf_auto2. }
+    mlSplitAnd.
+    * mlIntro. mlApplyMeta forall_equiv_1. mlAssumption.
+    * mlIntro. mlApplyMeta forall_equiv_2. mlAssumption.
+  Defined.
+
+  Theorem kore_equals_elim :
+    forall φ ψ (C : PatternCtx) s1 s2,
+      well_formed φ ->
+      well_formed ψ ->
+      well_formed s1 ->
+      well_formed s2 ->
+      PC_wf C ->
+      pattern_kt_well_formed (pcPattern C) ->
+      Γ ⊢ φ =ml(s1, s2) ψ --->
+          emplace C (φ ∷ s1) --->
+          emplace C (ψ ∷ s1) ∷ s2.
+  Proof.
+    intros.
+    unfold PC_wf in H3.
+    toMLGoal. wf_auto2.
+    mlIntro "H".
+    mlApplyMeta equals_equiv_1 in "H".
+    mlDestructAnd "H" as "H0" "Hsort".
+    mlIntro "HC".
+    mlSplitAnd. 2: mlAssumption.
+    pose proof (HEQ := equality_elimination Γ (φ ∷ s1) (ψ ∷ s1) C ltac:(unfold KoreTheory in HΓ;set_solver) ltac:(wf_auto2) ltac:(wf_auto2) ltac:(wf_auto2) H4).
+    mlApplyMeta HEQ.
+    mlSplitAnd; mlAssumption.
+  Defined.
+
+End Lemmas.
+
+Section countermodel_equal.
+
+(*   Context {Σ : Signature}
+          {S : Syntax}
+          {Γ : Theory}
+          (HΓ : KoreTheory ⊆ Γ). *)
+
+  Inductive syms := X_sym | Y_sym | def_sym | inh_sym | sorts_sym | s1_sym | s2_sym | next_sym | dv_sym | inj_sym.
+  Instance syms_eqdec : EqDecision syms.
+  Proof. solve_decision. Defined.
+  Program Instance syms_Finite : Finite syms.
+  Next Obligation.
+    exact ([X_sym; Y_sym; def_sym; inh_sym; sorts_sym; s1_sym; s2_sym; next_sym; dv_sym; inj_sym]).
+  Defined.
+  Next Obligation.
+    compute_done.
+  Defined.
+  Next Obligation.
+    destruct x; try compute_done.
+  Defined.
+
+
+  Program Instance KoreSig : Signature := {|
+    variables := StringMLVariables;
+    ml_symbols := {|
+      symbols := syms;
+    |};
+  |}.
+
+  Inductive carrier := a | b | c | def | inh | s1 | s2 | sorts.
+  Instance asd : Inhabited carrier.
+  Proof.
+    constructor. exact a.
+  Defined.
+
+(*   Definition sym_eval (s : syms) : propset syms :=
+    match s with
+    | X_sym => {[a ; b]}
+    | Y_sym => {[a ; c]}
+    end. *)
+
+  Program Definition KoreModel : @Model KoreSig :=
+    {|
+      Domain := carrier;
+    |}.
+  Next Obligation.
+    intros x y.
+    destruct x eqn:P.
+    * exact ∅.
+    * exact ∅.
+    * exact ∅.
+    * exact ⊤.
+    * destruct y eqn:Q.
+      - exact ∅.
+      - exact ∅.
+      - exact ∅.
+      - exact ∅.
+      - exact ∅.
+      - exact {[a]}.
+      - exact {[a;b;c]}.
+      - exact {[s1; s2]}.
+    * exact ∅.
+    * exact ∅.
+    * exact ∅.
+  Defined.
+  Next Obligation.
+    intros s. destruct s eqn:P.
+    * exact {[a; b]}.
+    * exact {[a; c]}.
+    * exact {[def]}.
+    * exact {[inh]}.
+    * exact {[sorts]}.
+    * exact {[s1]}.
+    * exact {[s2]}.
+    * exact ∅.
+    * exact ∅.
+    * exact ∅.
+  Defined.
+  Fail Next Obligation.
+
+  Import Notations.
+
+  Program Instance Syn : Syntax.
+  Next Obligation.
+    intros x. destruct x eqn:P.
+    * exact next_sym.
+    * exact dv_sym.
+    * exact inj_sym.
+  Defined.
+  Next Obligation.
+    constructor.
+    * intros x. destruct x eqn:P.
+      - exact inh_sym.
+      - exact sorts_sym.
+    * constructor. intros. exact def_sym.
+  Defined.
+
+  Local Goal
+    forall ρ,
+      @eval _ KoreModel ρ (patt_sym X_sym =ml(patt_sym s1_sym, patt_sym s2_sym) patt_sym Y_sym) = {[a;b;c]}.
+  Proof.
+    Search LeibnizEquiv propset.
+    pose proof (@propset_leibniz_equiv _ KoreModel).
+    intros.
+    unfold kore_equals, kore_iff, kore_implies, kore_ceil, kore_floor, kore_not, kore_and, kore_or, kore_cast, kore_top.
+    repeat rewrite eval_simpl.
+    simpl.
+    repeat rewrite app_ext_singleton.
+    repeat rewrite union_empty_l_L.
+    do 10 rewrite union_empty_r_L.
+    do 8 rewrite union_empty_r_L.
+    simpl.
+    repeat rewrite Compl_Compl_propset.
+    assert ((⊤ ∖ {[a; b; c]} ∪ ∅ = ({[def;inh;s1;s2;sorts]} : propset KoreModel))). {
+      rewrite union_empty_r_L.
+      apply set_eq; intros; destruct x; split; intros; set_solver.
+    }
+    repeat rewrite H0.
+    repeat rewrite Compl_Compl_propset.
+    apply set_eq; intros; destruct x; split; intros; try set_solver.
+    * apply elem_of_compl; intro X.
+      apply elem_of_union in X as [X | X].
+      - 
+      - set_solver.
+    *
+    *
+  Qed.
+
+  Local Goal
+    forall ρ,
+      @eval _ KoreModel ρ (patt_sym X_sym =ml(patt_sym s2_sym, patt_sym s2_sym) patt_sym Y_sym) ≠ ⊤.
+
+End countermodel_equal.
+
