matching-logic/src/Tests/TEST_LocallyNameless.v
@@ -105,6 +105,7 @@ Module test_2.
     {|
       enum := [sym_c; sym_zero; sym_succ; sym_SortNat;
         sym_import_sorts Sorts_Syntax.sym_inh;
+        sym_import_sorts Sorts_Syntax.sym_sorts;
         sym_import_definedness Definedness_Syntax.def_sym] ;
     |}.
     Next Obligation.
@@ -276,10 +277,10 @@ Module test_3.
       Γₙₐₜ ⊢i sym_tt ∈ml sym_even ⋅ (sym_succ ⋅ (sym_succ ⋅ (sym_succ ⋅ (sym_succ ⋅ sym_zero)))) using AnyReasoning.
     Proof.
       assert (Γₙₐₜ ⊢i ruleA using AnyReasoning) as RA.
-      { pose proof BasicProofSystemLemmas.hypothesis. gapply hypothesis; [ apply pile_any | wf_auto2 | set_solver ]. } 
+      { pose proof hypothesis. gapply hypothesis; [ apply pile_any | wf_auto2 | set_solver ]. } 
       (* TODO: <- create a tactic for the previous assertion *)
       assert (Γₙₐₜ ⊢i ruleC using AnyReasoning) as RC.
-      { gapply BasicProofSystemLemmas.hypothesis; [ apply pile_any | wf_auto2 | set_solver ]. }
+      { gapply hypothesis; [ apply pile_any | wf_auto2 | set_solver ]. }
       apply universal_generalization with (x := "X") in RA as RA1. (* revert Meta *)
       2: apply pile_any. 2: auto.
       unfold ruleA in RA1.
