matching-logic/src/Theories/Sorts_ProofSystem.v
@@ -46,8 +46,8 @@ Proof.
 
   unfold nest_ex; simpl.
 
-  remember (fresh_evar (b0 ∈ml 〚 patt_sym s 〛 and ϕ)) as x.
-  rewrite <- evar_quantify_evar_open with (n := 0) (x := x) (phi := b0 ∈ml 〚 patt_sym s 〛 and ϕ).
+  remember (fresh_evar (b0 ∈ml ⟦ patt_sym s ⟧ and ϕ)) as x.
+  rewrite <- evar_quantify_evar_open with (n := 0) (x := x) (phi := b0 ∈ml ⟦ patt_sym s ⟧ and ϕ).
   2: {
     subst x. eapply evar_is_fresh_in_richer'.
     2: apply set_evar_fresh_is_fresh'.
@@ -57,7 +57,7 @@ Proof.
     wf_auto2.
   }
 
-  gapply BasicProofSystemLemmas.Ex_gen.
+  gapply Ex_gen.
   { apply pile_any. }
   { apply pile_any. }
   {
@@ -74,7 +74,7 @@ Proof.
   mlDestructAnd "H" as "H0" "H1".
   mlClear "H0".
 
-  mlApplyMeta BasicProofSystemLemmas.Ex_quan. simpl.
+  mlApplyMeta Ex_quan. simpl.
   mlExact "H1".
 Defined.
 
